lang/Cfg.dfy
@@ -11,6 +11,15 @@ module BoogieCfg {
   type BlockId = nat 
 
   datatype Cfg = Cfg(entry: BlockId, blocks: map<BlockId, BasicBlock>, successors: map<BlockId, seq<BlockId>>)
+  /* TODO
+  {
+    function method ToString(n: BlockId) : string
+    {
+      if n in blocks.Keys then
+        ""
+    }
+  }
+  */
 
   predicate GraphWf<T>(succRel: map<T, seq<T>>)
   {
