transformations/AllTransformations.dfy
@@ -35,18 +35,27 @@ module AllTransformations
 
     LoopElim.EliminateLoopsPreserveNoBreaks(c);
 
+    print("=====After loop elimination=====\n");
+    print(c1.ToString(0));
+
     /** Eliminate if guards */
     var c2 := IfGuardElim.EliminateIfGuards(c1); 
+    print("=====After If guard elimination=====\n");
+    print(c2.ToString(0));
 
     IfGuardElim.EliminateIfGuardsNoLoops(c1);
 
     /** Remove scoped variables */
     var (c3, decls3) := DesugarScopedVarsImpl.RemoveScopedVars(c2);
     DesugarScopedVarsImpl.RemoveScopedVarsStructure(c2);
+    print("=====After removing scoped variables=====\n");
+    print(c3.ToString(0));
 
     /** Normalize AST */
     var (c4Opt, scExitOpt) := NormalizeAst.NormalizeAst(c3, None);
     var c4 := NormalizeAst.SeqCmdSimpleOpt(c4Opt, scExitOpt);
+    print("=====After AST normalization=====\n");
+    print(c4.ToString(0));
 
     NormalizeAst.NormalizeAstPreserveStructure(c3, None);
 
@@ -72,6 +81,14 @@ module AllTransformations
     var g2 := Passification.PassifyCfg(g1, topo, pred);
 
     /** VCGen */
+    if |topo| == 0 {
+      print("no blocks");
+    } else {
+      print("g1:\n");
+      print(g1.blocks[topo[0]].ToString(0));
+      print("\n g2:\n");
+      print(g2.blocks[topo[0]].ToString(0));
+    }
 
     var vc := 
       if |topo| == 0 then
@@ -81,5 +98,26 @@ module AllTransformations
 
     return vc;
   }
+  
+}
 
+import opened BoogieLang
+import opened Wrappers
+
+method Main()
+{
+  var c := 
+    Scope(
+      None,
+      [("x", TPrim(TInt))], 
+      Seq(
+        SimpleCmd(Assume(BinOp(Var("x"), Gt, ELit(LitInt(0))))),
+        SimpleCmd(Assert(BinOp(Var("x"), Gt, ELit(LitInt(0)))))
+      )
+    );
+  
+  var vc := AllTransformations.AllTransformations(c);
+  var vcString := vc.ToString();
+
+  print(vcString);
 }
